Add optimization for generic recognizer

src/Parsers/GenericRecognizerOptimized.v
@@ -34,6 +34,7 @@ Require Export Fiat.Common.NatFacts.
 Require Export Fiat.Common.Sigma.
 Require Import Fiat.Parsers.StringLike.Core.
 Require Import Fiat.Parsers.StringLike.Properties.
+Require Import Fiat.Parsers.GenericRecognizerOptimizedTactics.
 Import NPeano.
 
 Set Implicit Arguments.
@@ -42,129 +43,9 @@ Local Open Scope string_like_scope.
 Global Arguments string_dec : simpl never.
 Global Arguments string_beq : simpl never.
 
-Module Export opt.
-  Module Import opt.
-    Definition first_index_default {A} := Eval compute in @Operations.List.first_index_default A.
-    Definition map {A B} := Eval compute in @List.map A B.
-    Definition length {A} := Eval compute in @List.length A.
-    Definition uniquize {A} := Eval compute in @Operations.List.uniquize A.
-    Definition string_beq := Eval compute in Equality.string_beq.
-    Definition option_rect {A} := Eval compute in @option_rect A.
-    Definition up_to := Eval compute in Operations.List.up_to.
-    Definition rev {A} := Eval compute in @List.rev A.
-    Definition combine {A B} := Eval compute in @List.combine A B.
-    Definition fold_left {A B} := Eval compute in @List.fold_left A B.
-    Definition fold_right {A B} := Eval compute in @List.fold_right A B.
-    Definition list_rect {A} := Eval compute in @list_rect A.
-    Definition hd {A} := Eval compute in @hd A.
-    Definition tl {A} := Eval compute in @tl A.
-    Definition nth {A} := Eval compute in @nth A.
-    Definition nth' {A} := Eval cbv beta iota zeta delta -[EqNat.beq_nat] in @nth' A.
-    Definition fst {A B} := Eval compute in @fst A B.
-    Definition snd {A B} := Eval compute in @snd A B.
-    Definition list_caset {A} := Eval compute in @list_caset A.
-    Definition item_rect {A} := Eval compute in @item_rect A.
-    Definition ritem_rect {A} := Eval compute in @ritem_rect A.
-    Definition bool_rect := Eval compute in bool_rect.
-    Definition pred := Eval compute in pred.
-    Definition minusr := Eval compute in minusr.
-    Definition id {A} := Eval compute in @id A.
-    Definition beq_nat := Eval compute in EqNat.beq_nat.
-    Definition leb := Eval compute in Compare_dec.leb.
-    Definition interp_RCharExpr {Char idata} := Eval cbv -[andb orb negb Compare_dec.leb] in @interp_RCharExpr Char idata.
-  End opt.
-
-  Declare Reduction opt_red := cbv beta iota zeta delta [first_index_default map length uniquize string_beq option_rect up_to rev combine fold_left fold_right list_rect hd tl Common.opt.fst Common.opt.snd nth nth' fst snd list_caset item_rect ritem_rect bool_rect pred minusr id beq_nat leb interp_RCharExpr].
-  Ltac opt_red x := eval opt_red in x.
-End opt.
-
-Module Export opt2.
-  Module Import opt2.
-    Definition first_index_default {A} := Eval compute in @Operations.List.first_index_default A.
-    Definition map {A B} := Eval compute in @List.map A B.
-    Definition length {A} := Eval compute in @List.length A.
-    Definition uniquize {A} := Eval compute in @Operations.List.uniquize A.
-    Definition string_beq := Eval compute in Equality.string_beq.
-    Definition option_rect {A} := Eval compute in @option_rect A.
-    Definition up_to := Eval compute in Operations.List.up_to.
-    Definition rev {A} := Eval compute in @List.rev A.
-    Definition combine {A B} := Eval compute in @List.combine A B.
-    Definition fold_left {A B} := Eval compute in @List.fold_left A B.
-    Definition fold_right {A B} := Eval compute in @List.fold_right A B.
-    Definition list_rect {A} := Eval compute in @list_rect A.
-    Definition hd {A} := Eval compute in @hd A.
-    Definition tl {A} := Eval compute in @tl A.
-    Definition nth {A} := Eval compute in @nth A.
-    Definition nth' {A} := Eval cbv beta iota zeta delta -[EqNat.beq_nat] in @nth' A.
-    Definition fst {A B} := Eval compute in @fst A B.
-    Definition snd {A B} := Eval compute in @snd A B.
-    Definition list_caset {A} := Eval compute in @list_caset A.
-    Definition item_rect {A} := Eval compute in @item_rect A.
-    Definition ritem_rect {A} := Eval compute in @ritem_rect A.
-    Definition bool_rect := Eval compute in bool_rect.
-    Definition pred := Eval compute in pred.
-    Definition minusr := Eval compute in minusr.
-    Definition id {A} := Eval compute in @id A.
-    Definition beq_nat := Eval compute in EqNat.beq_nat.
-    Definition leb := Eval compute in Compare_dec.leb.
-    Definition interp_RCharExpr {Char idata} := Eval cbv -[andb orb negb Compare_dec.leb] in @interp_RCharExpr Char idata.
-  End opt2.
-
-  Declare Reduction opt2_red := cbv beta iota zeta delta [first_index_default map length uniquize string_beq option_rect up_to rev combine fold_left fold_right list_rect hd tl Common.opt.fst Common.opt.snd nth nth' fst snd list_caset item_rect ritem_rect bool_rect pred minusr id beq_nat leb interp_RCharExpr].
-  Ltac opt2_red x := eval opt2_red in x.
-End opt2.
-
-Module Export opt3.
-  Module Import opt3.
-    Definition first_index_default {A} := Eval compute in @Operations.List.first_index_default A.
-    Definition map {A B} := Eval compute in @List.map A B.
-    Definition length {A} := Eval compute in @List.length A.
-    Definition uniquize {A} := Eval compute in @Operations.List.uniquize A.
-    Definition string_beq := Eval compute in Equality.string_beq.
-    Definition option_rect {A} := Eval compute in @option_rect A.
-    Definition up_to := Eval compute in Operations.List.up_to.
-    Definition rev {A} := Eval compute in @List.rev A.
-    Definition combine {A B} := Eval compute in @List.combine A B.
-    Definition fold_left {A B} := Eval compute in @List.fold_left A B.
-    Definition fold_right {A B} := Eval compute in @List.fold_right A B.
-    Definition list_rect {A} := Eval compute in @list_rect A.
-    Definition hd {A} := Eval compute in @hd A.
-    Definition tl {A} := Eval compute in @tl A.
-    Definition nth {A} := Eval compute in @nth A.
-    Definition nth' {A} := Eval cbv beta iota zeta delta -[EqNat.beq_nat] in @nth' A.
-    Definition fst {A B} := Eval compute in @fst A B.
-    Definition snd {A B} := Eval compute in @snd A B.
-    Definition list_caset {A} := Eval compute in @list_caset A.
-    Definition item_rect {A} := Eval compute in @item_rect A.
-    Definition ritem_rect {A} := Eval compute in @ritem_rect A.
-    Definition bool_rect := Eval compute in bool_rect.
-    Definition pred := Eval compute in pred.
-    Definition minusr := Eval compute in minusr.
-    Definition id {A} := Eval compute in @id A.
-    Definition beq_nat := Eval compute in EqNat.beq_nat.
-    Definition leb := Eval compute in Compare_dec.leb.
-    Definition interp_RCharExpr {Char idata} := Eval cbv -[andb orb negb Compare_dec.leb] in @interp_RCharExpr Char idata.
-  End opt3.
-
-  Declare Reduction opt3_red := cbv beta iota zeta delta [first_index_default map length uniquize string_beq option_rect up_to rev combine fold_left fold_right list_rect hd tl Common.opt.fst Common.opt.snd nth nth' fst snd list_caset item_rect ritem_rect bool_rect pred minusr id beq_nat leb interp_RCharExpr].
-  Ltac opt3_red x := eval opt3_red in x.
-End opt3.
-
 Section recursive_descent_parser.
   Context {Char} {HSLM : StringLikeMin Char} {HSL : StringLike Char}
           {G : pregrammar Char}.
-
-  (*Let HNoDup' : NoDupR (fun x y => string_beq (fst x) (fst y)) (pregrammar_productions G).
-  Proof.
-    pose proof (nonterminals_unique G) as HNoDup.
-    hnf in HNoDup |- *; unfold pregrammar_nonterminals in *; simpl in *.
-    rewrite uniquize_map in HNoDup.
-    apply uniquize_length.
-    apply (f_equal (@List.length _)) in HNoDup.
-    rewrite !map_length in HNoDup.
-    rewrite !map_length, <- HNoDup; clear HNoDup.
-    reflexivity.
-  Qed.*)
 
   Context (Hvalid : is_true (grammar_rvalid G)).
 
@@ -193,6 +74,16 @@ Section recursive_descent_parser.
       parse_nt_is_correct str (of_nonterminal nt) b pnt
       <-> parse_nt_is_correct str (of_nonterminal nt) b (parse_nonterminal (data := data) str nt).
 
+  Local Arguments Compare_dec.leb !_ !_.
+  Local Arguments to_nonterminal / .
+
+  Local Instance good_nth_proper {A}
+  : Proper (eq ==> _ ==> _ ==> eq) (nth (A:=A))
+    := _.
+  Local Instance good_nth'_proper {A}
+  : Proper (eq ==> _ ==> _ ==> eq) (nth' (A:=A))
+    := _.
+
   Lemma parse_nonterminal_optdata_eq
         {HSLP : StringLikeProperties Char}
         {splitdata_correct : @boolean_parser_completeness_dataT' _ _ _ G data}
@@ -209,647 +100,6 @@ Section recursive_descent_parser.
         try solve [ tauto
                   | exfalso; eauto using @parse_nt_is_correct_disjoint ].
   Qed.
-
-  Local Ltac contract_drop_take_t :=
-    idtac;
-    match goal with
-      | [ H : is_true (bool_eq ?x ?y) |- _ ] => change (beq x y) in H
-      | [ H : context[is_true (bool_eq ?x ?y)] |- _ ] => change (is_true (bool_eq x y)) with (beq x y) in H
-      | [ |- context[is_true (bool_eq ?x ?y)] ] => change (is_true (bool_eq x y)) with (beq x y)
-      | _ => progress subst
-      | [ H : beq _ _ |- _ ] => rewrite !H; clear H
-      | [ |- _ = _ ] => reflexivity
-      | [ |- beq _ _ ] => reflexivity
-      | [ |- Equivalence _ ] => split; repeat intro
-    end.
-
-  Local Ltac t_reduce_fix :=
-    repeat match goal with
-             | _ => progress simpl sumbool_rect
-             | _ => progress simpl option_rect
-             | [ |- context[lt_dec ?x ?y] ]
-               => destruct (lt_dec x y)
-             | [ |- context[dec ?x] ]
-               => destruct (dec x)
-             | [ |- @fold_right ?A ?B ?f ?x ?ls = @fold_right ?A ?B ?f ?x ?ls' ]
-               => apply (_ : Proper (_ ==> _ ==> _ ==> eq) (@fold_right A B))
-             | [ |- @fold_left ?A ?B ?f ?ls ?x = @fold_left ?A ?B ?f ?ls' ?x ]
-               => apply (_ : Proper (_ ==> _ ==> _ ==> eq) (@fold_left A B))
-             | [ |- @list_caset ?A (fun _ => ?P) _ _ ?ls = @list_caset ?A (fun _ => ?P) _ _ ?ls' ]
-               => apply (_ : Proper (_ ==> pointwise_relation _ (pointwise_relation _ _) ==> _ ==> eq) (@list_caset A (fun _ => P)))
-             | [ |- @map ?A ?B ?f ?ls = @map ?A ?B ?f' ?ls' ]
-               => apply (_ : Proper (pointwise_relation _ _ ==> _ ==> eq) (@map A B))
-             | [ |- @nth' ?A ?n ?ls ?d = @nth' ?A ?n' ?ls' ?d' ]
-               => apply f_equal3
-             | [ |- @nth ?A ?n ?ls ?d = @nth ?A ?n' ?ls' ?d' ]
-               => apply f_equal3
-             | _ => intro
-             | [ |- ?x = ?x ] => reflexivity
-             | [ |- bool_rect ?P _ _ ?b = bool_rect ?P _ _ ?b ] => apply f_equal3
-             | [ |- andb _ _ = andb _ _ ] => apply f_equal2
-             | [ |- andbr _ _ = andbr _ _ ] => apply f_equal2
-             | [ |- orb _ _ = orb _ _ ] => apply f_equal2
-             | [ |- ret_nt _ = ret_nt _ ] => apply f_equal
-             | [ |- ret_NonTerminal_true _ _ = ret_NonTerminal_true _ _ ] => apply f_equal
-             | [ |- ret_production_cons _ _ = ret_production_cons _ _ ] => apply f_equal2
-             | [ |- match ?it with Terminal _ => _ | _ => _ end = match ?it with _ => _ end ] => is_var it; destruct it
-             | [ |- context[(fst ?x, snd ?x)] ] => rewrite <- !surjective_pairing
-             | [ |- context[andb _ true] ] => rewrite Bool.andb_true_r
-             | [ |- context[andb true _] ] => rewrite Bool.andb_true_l
-             | [ |- context[andb _ false] ] => rewrite Bool.andb_false_r
-             | [ |- context[andb false _] ] => rewrite Bool.andb_false_l
-             | [ |- context[andb ?x true] ] => rewrite (andbr_andb x true)
-             | [ |- context[andb true _] ] => rewrite (andbr_andb true)
-             | [ |- context[andb ?x false] ] => rewrite (andbr_andb x false)
-             | [ |- context[andbr false _] ] => rewrite (andbr_andb false)
-             | [ |- context[orb _ true] ] => rewrite Bool.orb_true_r
-             | [ |- context[orb true _] ] => rewrite Bool.orb_true_l
-             | [ |- context[orb _ false] ] => rewrite Bool.orb_false_r
-             | [ |- context[orb false _] ] => rewrite Bool.orb_false_l
-             | [ |- cons _ _ = cons _ _ ]
-               => apply f_equal2
-             | _ => solve [ auto with nocore ]
-             | [ |- prod_relation lt lt _ _ ] => hnf; simpl; omega
-             | [ H : (_ && _)%bool = true |- _ ] => apply Bool.andb_true_iff in H
-             | [ H : _ = in_left |- _ ] => clear H
-             | [ H : _ /\ _ |- _ ] => destruct H
-             | [ H : context[negb (EqNat.beq_nat ?x ?y)] |- _ ] => destruct (EqNat.beq_nat x y) eqn:?
-             | [ H : EqNat.beq_nat _ _ = false |- _ ] => apply EqNat.beq_nat_false in H
-             | [ H : EqNat.beq_nat _ _ = true |- _ ] => apply EqNat.beq_nat_true in H
-             | [ H : snd ?x = _ |- _ ] => is_var x; destruct x
-             | _ => progress simpl negb in *
-             | [ H : false = true |- _ ] => inversion H
-             | [ |- ?f _ (match ?p with eq_refl => ?k end) = ?f' _ ?k ]
-               => destruct p
-             | [ |- match ?ls with nil => _ | _ => _ end = match ?ls with _ => _ end ]
-               => destruct ls eqn:?
-             | [ |- match ?ls with NonTerminal _ => _ | _ => _ end = match ?ls with _ => _ end ]
-               => destruct ls eqn:?
-             | [ |- match ?ls with RNonTerminal _ => _ | _ => _ end = match ?ls with _ => _ end ]
-               => destruct ls eqn:?
-             | [ |- (if ?e then _ else _) = (if ?e then _ else _) ]
-               => destruct e eqn:?
-             | _ => solve [ intuition ]
-             | [ H : appcontext[sub_nonterminals_listT] |- _ ]
-               => solve [ apply H;
-                          intuition;
-                          (etransitivity; [ | eapply sub_nonterminals_listT_remove_2; eassumption ]); simpl;
-                          unfold remove_nonterminal; simpl;
-                          unfold rdp_list_remove_nonterminal;
-                          reflexivity ]
-           end.
-
-  Local Ltac t_reduce_list :=
-    idtac;
-    lazymatch goal with
-    | [ |- list_rect ?P ?n ?c ?ls ?idx ?offset ?len = list_rect ?P' ?n' ?c' ?ls ?idx ?offset ?len ]
-      => let n0 := fresh in
-         let c0 := fresh in
-         let n1 := fresh in
-         let c1 := fresh in
-         set (n0 := n);
-         set (n1 := n');
-         set (c0 := c);
-         set (c1 := c');
-         refine (list_rect
-                   (fun ls' => forall idx' offset' len', list_rect P n0 c0 ls' idx' offset' len' = list_rect P' n1 c1 ls' idx' offset' len')
-                   _
-                   _
-                   ls
-                   idx
-                   offset len);
-         simpl list_rect;
-         [ subst n0 c0 n1 c1; cbv beta
-         | intros; unfold c0 at 1, c1 at 1 ]
-    end.
-
-  Local Ltac t_reduce_list_generalize :=
-    idtac;
-    match goal with
-      | [ |- list_rect ?P ?n ?c ?ls ?offset ?len ?y = list_rect ?P' ?n' ?c' ?ls ?offset ?len ?y ]
-        => let n0 := fresh in
-           let c0 := fresh in
-           let n1 := fresh in
-           let c1 := fresh in
-           set (n0 := n);
-             set (n1 := n');
-             set (c0 := c);
-             set (c1 := c');
-             refine (list_rect
-                       (fun ls' => forall offset' len' y', list_rect P n0 c0 ls' offset' len' y' = list_rect P' n1 c1 ls' offset' len' y')
-                       _
-                       _
-                       ls
-                       offset len y);
-             simpl list_rect;
-             [ subst n0 c0 n1 c1; cbv beta
-             | intros; unfold n0 at 1, c0 at 1, n1 at 1, c1 at 1 ]
-    end.
-
-  Local Ltac refine_Fix2_5_Proper_eq :=
-    idtac;
-    (lazymatch goal with
-    | [ |- context[_ = @Fix2 ?A ?A' ?R ?Rwf ?T (fun a0 b0 c0 d0 e0 h0 i0 => @?f a0 b0 c0 d0 e0 h0 i0) ?a ?a' ?b ?c ?d ?e ?h] ]
-      => (lazymatch T with
-         | (fun a' : ?A0 => forall (b' :@?B a') (c' : @?C a' b') (d' : @?D a' b' c') (e' : @?E a' b' c' d') (h' : @?H a' b' c' d' e'), @?P a' b' c' d' e' h')
-           => let H' := fresh in
-              (*refine (_ : @Fix A R Rwf T (fun a0 b0 c0 d0 e0 h0 i0 => _) a b c d e h = _);
-                 let f' := match goal with |- @Fix _ _ _ _ ?f' _ _ _ _ _ _ = _ => constr:(f') end in*)
-              pose proof ((fun f' H0 => @Fix2_5_Proper_eq A A' B C D E H R Rwf P f' f H0 a a' b c d e h)) as H';
-          cbv beta in H';
-          (lazymatch type of H' with
-          | forall f' : ?f'T, @?H'T f' -> _
-            => let H'' := fresh in
-               let f'' := fresh in
-               assert (H'' : { f' : f'T & H'T f' });
-           [ clear H'
-           | destruct H'' as [f'' H''];
-             specialize (H' f'' H'');
-             clear H''; eexists; exact H' ]
-           end)
-          end)
-     end);
-    unfold forall_relation, pointwise_relation, respectful;
-    cbv beta;
-    eexists (fun a0 a0' b0 c0 d0 e0 h0 i0 => _); intros.
-
-  Local Ltac refine_Fix2_5_Proper_eq_with_assumptions' HP HPpf :=
-    idtac;
-      (lazymatch goal with
-        | [ |- context[_ = @Fix2 ?A ?A' ?R ?Rwf ?T (fun a0 b0 c0 d0 e0 h0 i0 => @?f a0 b0 c0 d0 e0 h0 i0) ?a ?a' ?b ?c ?d ?e ?h] ]
-          => (lazymatch T with
-               | (fun a' : ?A0 => forall (b' :@?B a') (c' : @?C a' b') (d' : @?D a' b' c') (e' : @?E a' b' c' d') (h' : @?H a' b' c' d' e'), @?P a' b' c' d' e' h')
-                 => let H' := fresh in
-                    pose proof ((fun f' H0 => @Fix2_5_Proper_eq_with_assumption A A' B C D E H R Rwf P HP f' f H0 a a' b c d e h HPpf)) as H';
-                    cbv beta in H';
-                    (lazymatch type of H' with
-                      | forall f' : ?f'T, @?H'T f' -> _
-                        => let H'' := fresh in
-                           let f'' := fresh in
-                           assert (H'' : { f' : f'T & H'T f' });
-                           [ clear H'
-                           | destruct H'' as [f'' H''];
-                             specialize (H' f'' H'');
-                             clear H''; eexists; exact H' ]
-                      end)
-               end)
-        end);
-      unfold forall_relation, pointwise_relation, respectful;
-      cbv beta;
-      eexists (fun a0 a0' b0 c0 d0 e0 h0 i0 => _); intros.
-
-  Local Ltac refine_Fix2_5_Proper_eq_with_assumptions :=
-    idtac;
-    let HPHPpf := lazymatch goal with
-        | [ |- appcontext[Fix2 _ _ (fun (a0 : ?A0) (b0 :@?B a0) (c0 : @?C a0 b0) (d0 : @?D a0 b0) (e0 : @?E a0 b0 d0) (h0 : @?H a0 b0 d0 e0) (i0 : @?I a0 b0 d0 e0 h0) (j0 : @?J a0 b0 d0 e0 h0 i0) => _) ?a ?b ?d ?e ?h ?i ?j] ]
-          => let HP := constr:(fun a0 b0 d0 e0 h0 i0 (j0 : J a0 b0 d0 e0 h0 i0) => sub_nonterminals_listT d0 initial_nonterminals_data /\ (a0 <= h0 \/ is_valid_nonterminal initial_nonterminals_data j0)) in
-             let HPpfT := (eval cbv beta in (HP a b d e h i j)) in
-             let HPpf := constr:(fun pf => conj pf (or_introl (reflexivity _)) : HPpfT) in
-             (eval cbv beta in (HP, HPpf))
-        end in
-    let HP := match HPHPpf with (?HP, ?HPpf) => HP end in
-    let HPpf := match HPHPpf with (?HP, ?HPpf) => HPpf end in
-    let T := match type of HPpf with ?T -> _ => T end in
-    let H0 := fresh "H" in
-    assert (H0 : T)
-      by (simpl; unfold rdp_list_initial_nonterminals_data, pregrammar'_of_pregrammar, pregrammar_productions; rewrite !map_length; reflexivity);
-    let HPpf := constr:(HPpf H0) in
-    refine_Fix2_5_Proper_eq_with_assumptions' HP HPpf.
-
-  Local Ltac fin_step_opt :=
-    repeat match goal with
-             | [ |- _ = true ] => reflexivity
-             | [ |- _ = false ] => reflexivity
-             | [ |- _ = ret_nt_invalid ] => reflexivity
-             | [ |- ?x = ?x ] => reflexivity
-             | [ |- _ = ?x ] => is_var x; reflexivity
-             | [ |- _ = (_::_) ] => apply (f_equal2 (@cons _))
-             | [ |- _ = nil ] => reflexivity
-             | [ |- _ = 0 ] => reflexivity
-             | [ |- _ = 1 ] => reflexivity
-             | [ |- _ = None ] => reflexivity
-             | [ |- _ = EqNat.beq_nat _ _ ] => apply f_equal2
-             | [ |- _ = Compare_dec.leb _ _ ] => apply f_equal2
-             | [ |- _ = S _ ] => apply f_equal
-             | [ |- _ = string_beq _ _ ] => apply f_equal2
-             | [ |- _ = fst ?x ] => is_var x; reflexivity
-             | [ |- _ = snd ?x ] => is_var x; reflexivity
-             | [ |- _ = pregrammar_productions ?x ] => is_var x; reflexivity
-             | [ |- _ = pregrammar_rproductions ?x ] => is_var x; reflexivity
-             | [ |- context[(0 - _)%natr] ] => rewrite (minusr_minus 0); simpl (minus 0)
-             | [ |- _ = (_, _) ] => apply f_equal2
-             | _ => progress cbv beta
-             | [ |- context[orb _ false] ] => rewrite Bool.orb_false_r
-             | [ |- context[orb _ true] ] => rewrite Bool.orb_true_r
-             | [ |- context[andbr _ false] ] => rewrite (andbr_andb _ false)
-             | [ |- context[andbr _ true] ] => rewrite (andbr_andb _ true)
-             | [ |- context[andb _ false] ] => rewrite Bool.andb_false_r
-             | [ |- context[andb _ true] ] => rewrite Bool.andb_true_r
-           end.
-
-  Local Ltac misc_opt' :=
-    idtac;
-    match goal with
-    | _ => progress rewrite ?max_min_n, ?Minus.minus_diag, ?Nat.sub_0_r, ?uneta_bool, ?beq_nat_min_0(*, ?bool_rect_flatten*)
-    | _ => rewrite Min.min_l by assumption
-    | _ => rewrite Min.min_r by assumption
-    | [ |- context[if ?ltb ?x ?y then _ else _] ] => rewrite if_to_min
-    | [ |- context[min ?x ?y - ?x] ] => rewrite min_sub_same
-    | [ |- context[(min ?x ?y - ?x)%natr] ] => rewrite min_subr_same
-    | [ |- context[?x - (?x - ?y)%natr] ]
-      => rewrite !(minusr_minus x y), sub_twice, <- ?minusr_minus
-    | _ => progress fin_step_opt
-    end.
-
-  Local Ltac misc_opt := set_evars; progress repeat misc_opt'; subst_evars.
-
-  Local Ltac step_opt' :=
-    idtac;
-    match goal with
-      | _ => rewrite <- !minusr_minus
-      | [ |- _ = @option_rect ?A ?B (fun s => _) _ _ ]
-        => refine (_ : @option_rect A B (fun s => _) _ _ = _);
-          apply (_ : Proper (pointwise_relation _ _ ==> _ ==> _ ==> eq) (@option_rect A B));
-          repeat intro
-      | [ |- _ = @bool_rect ?A _ _ _ ]
-        => refine (_ : @bool_rect A _ _ _ = _);
-          apply (_ : Proper (_ ==> _ ==> _ ==> eq) (@bool_rect A));
-          repeat intro
-      | [ |- _ = fold_right orb false _ ]
-        => rewrite <- !(@fold_symmetric _ orb) by first [ apply Bool.orb_assoc | apply Bool.orb_comm ]
-      | [ |- _ = @fold_left ?A ?B orb _ false ]
-        => refine (_ : fold_left orb _ false = _);
-          apply (_ : Proper (_ ==> _ ==> _ ==> _) (@fold_left A B)); repeat intro
-      | [ |- _ = @fold_left ?A ?B orbr _ false ]
-        => refine (_ : fold_left orbr _ false = _);
-          apply (_ : Proper (_ ==> _ ==> _ ==> _) (@fold_left A B)); repeat intro
-      | [ |- _ = @fold_right ?A ?B (fun x y => _) _ _ ]
-        => refine (_ : fold_right (fun x y => _) _ _ = _);
-          apply (_ : Proper (_ ==> _ ==> _ ==> _) (@fold_right A B)); repeat intro
-      | [ |- _ = @map ?A ?B _ _ ]
-        => refine (_ : @map A B (fun x => _) _ = _);
-          apply (_ : Proper (pointwise_relation _ _ ==> _ ==> _) (@map A B)); repeat intro
-      | [ |- _ = @list_caset ?A ?P _ _ _ ]
-        => refine (_ : @list_caset A P _ _ _ = _);
-          apply (_ : Proper (forall_relation _ ==> forall_relation (fun _ => forall_relation _) ==> forall_relation _) (@list_caset A P)); repeat intro
-      | [ |- _ = @list_caset ?A (fun _ => ?P) _ _ _ ]
-        => refine (_ : @list_caset A (fun _ => P) _ _ _ = _);
-          apply (_ : Proper (_ ==> pointwise_relation _ (pointwise_relation _ _) ==> _ ==> _) (@list_caset A (fun _ => P))); repeat intro
-      | [ |- _ = @nth ?A _ _ _ ]
-        => rewrite <- nth'_nth
-      | [ |- _ = @nth' ?A _ _ _ ]
-        => refine (_ : @nth' A _ _ _ = _);
-          apply f_equal3
-      | [ |- _ = sumbool_rect ?T ?A ?B ?c ]
-        => let A' := fresh in
-           let B' := fresh in
-           let TA := type of A in
-           let TB := type of B in
-           evar (A' : TA); evar (B' : TB);
-           refine (sumbool_rect
-                     (fun c' => sumbool_rect T A' B' c' = sumbool_rect T A B c')
-                     _ _ c); intro; subst A' B'; simpl @sumbool_rect
-      | [ |- ?e = match ?ls with nil => _ | _ => _ end ]
-        => is_evar e; refine (_ : match ls with nil => _ | _ => _ end = _)
-      | [ |- match ?ls with nil => ?A | x::xs => @?B x xs end = match ?ls with nil => ?A' | x::xs => @?B' x xs end ]
-        => refine (match ls
-                         as ls'
-                         return match ls' with nil => A | x::xs => B x xs end = match ls' with nil => A' | x::xs => B' x xs end
-                   with
-                     | nil => _
-                     | _ => _
-                   end)
-      | [ |- _ = item_rect ?T ?A ?B ?c ] (* evar kludge following *)
-        => revert c;
-          let RHS := match goal with |- forall c', _ = ?RHS c' => RHS end in
-          let f := constr:(fun TC NC =>
-                             forall c, item_rect T TC NC c = RHS c) in
-          let f := (eval cbv beta in f) in
-          let e1 := fresh in
-          let e2 := fresh in
-          match type of f with
-            | ?X -> ?Y -> _
-              => evar (e1 : X); evar (e2 : Y)
-          end;
-            intro c;
-            let ty := constr:(item_rect T e1 e2 c = RHS c) in
-            etransitivity_rev _; [ refine (_ : ty) | reflexivity ];
-            revert c;
-            refine (item_rect
-                      (fun c => item_rect T e1 e2 c = RHS c)
-                      _ _);
-            intro c; simpl @item_rect; subst e1 e2
-      | [ |- _ = ritem_rect ?T ?A ?B ?c ] (* evar kludge following *)
-        => revert c;
-          let RHS := match goal with |- forall c', _ = ?RHS c' => RHS end in
-          let f := constr:(fun TC NC =>
-                             forall c, ritem_rect T TC NC c = RHS c) in
-          let f := (eval cbv beta in f) in
-          let e1 := fresh in
-          let e2 := fresh in
-          match type of f with
-            | ?X -> ?Y -> _
-              => evar (e1 : X); evar (e2 : Y)
-          end;
-            intro c;
-            let ty := constr:(ritem_rect T e1 e2 c = RHS c) in
-            etransitivity_rev _; [ refine (_ : ty) | reflexivity ];
-            revert c;
-            refine (ritem_rect
-                      (fun c => ritem_rect T e1 e2 c = RHS c)
-                      _ _);
-            intro c; simpl @ritem_rect; subst e1 e2
-      | [ |- _ = match ?x with true => true | false => false end ]
-        => transitivity x; [ | destruct x; reflexivity ]
-      | [ |- _ = ret_nt _ ]
-        => refine (_ : ret_nt _ = _);
-           refine (f_equal ret_nt _)
-      | [ |- _ = ret_NonTerminal_true ?x _ ]
-        => refine (_ : ret_NonTerminal_true x _ = _);
-           refine (f_equal (ret_NonTerminal_true x) _)
-      | [ |- _ = fold_right ret_orb_productions ?init ?ls ]
-        => rewrite <- (rev_involutive ls), fold_left_rev_right
-      | [ |- _ = fold_right ret_orb_production ?init ?ls ]
-        => rewrite <- (rev_involutive ls), fold_left_rev_right
-      | [ |- _ = @fold_left ?A ?B ?orb _ ret_orb_productions_base ]
-        => refine (_ : fold_left orb _ ret_orb_productions_base = _);
-           apply (_ : Proper (_ ==> _ ==> _ ==> _) (@fold_left A B)); repeat intro
-      | [ |- _ = @fold_left ?A ?B ?orb _ ret_orb_production_base ]
-        => refine (_ : fold_left orb _ ret_orb_production_base = _);
-           apply (_ : Proper (_ ==> _ ==> _ ==> _) (@fold_left A B)); repeat intro
-      | [ |- _ = rev (map _ _) ]
-        => rewrite <- map_rev
-    end;
-    fin_step_opt.
-
-  Local Ltac step_opt := repeat step_opt'.
-
-  Local Ltac sigL_transitivity term :=
-    idtac;
-    (lazymatch goal with
-    | [ |- ?sig (fun x : ?T => @?A x = ?B) ]
-      => (let H := fresh in
-          let H' := fresh in
-          assert (H : sig (fun x : T => A x = term));
-          [
-          | assert (H' : term = B);
-            [ clear H
-            | let x' := fresh in
-              destruct H as [x' H];
-                exists x'; transitivity term; [ exact H | exact H' ] ] ])
-     end).
-
-  Local Ltac fix_trans_helper RHS x y :=
-    match RHS with
-      | appcontext G[y] => let RHS' := context G[x] in
-                           fix_trans_helper RHS' x y
-      | _ => constr:(RHS)
-    end.
-
-  Local Ltac fix2_trans :=
-    match goal with
-      | [ H : forall a0 a0' a1 a2 a3 a4 a5 a6, ?x a0 a0' a1 a2 a3 a4 a5 a6 = ?y a0 a0' a1 a2 a3 a4 a5 a6 |- _ = ?RHS ]
-        => let RHS' := fix_trans_helper RHS x y
-           in transitivity RHS'; [ clear H y | ]
-    end.
-
-  Local Ltac fix2_trans_with_assumptions :=
-    match goal with
-      | [ H : forall a0 a0' a1 a2 a3 a4 a5 a6, _ -> ?x a0 a0' a1 a2 a3 a4 a5 a6 = ?y a0 a0' a1 a2 a3 a4 a5 a6 |- _ = ?RHS ]
-        => let RHS' := fix_trans_helper RHS x y
-           in transitivity RHS'; [ clear H y | ]
-    end.
-
-  Local Ltac t_prereduce_list_evar :=
-    idtac;
-    let RHS := match goal with |- _ = ?RHS => RHS end in
-    lazymatch RHS with
-    | appcontext RHS'[list_rect ?P ?f ?g]
-      => let ft := type of f in
-         let gt := type of g in
-         let f' := fresh in
-         let g' := fresh in
-         evar (f' : ft); evar (g' : gt);
-         let f0 := (eval unfold f' in f') in
-         let g0 := (eval unfold g' in g') in
-         let RHS'' := context RHS'[list_rect P f0 g0] in
-         refine (_ : RHS'' = _)
-    end.
-
-  Local Ltac t_postreduce_list :=
-    idtac;
-    lazymatch goal with
-      | [ |- list_rect ?P ?N ?C ?ls ?a ?b ?c = list_rect ?P ?N' ?C' ?ls ?a ?b ?c ]
-        => let P0 := fresh in
-           let N0 := fresh in
-           let C0 := fresh in
-           let N1 := fresh in
-           let C1 := fresh in
-           set (P0 := P);
-             set (N0 := N);
-             set (C0 := C);
-             set (N1 := N');
-             set (C1 := C');
-             let IH := fresh "IH" in
-             let xs := fresh "xs" in
-             refine (list_rect
-                       (fun ls' => forall a' b' c',
-                                     list_rect P0 N0 C0 ls' a' b' c'
-                                     = list_rect P0 N1 C1 ls' a' b' c')
-                       _
-                       _
-                       ls a b c);
-               simpl @list_rect;
-               [ subst P0 N0 C0 N1 C1; intros; cbv beta
-               | intros ? xs IH; intros; unfold C0 at 1, C1 at 1; cbv beta;
-                 setoid_rewrite <- IH; clear IH N1 C1;
-                 generalize (list_rect P0 N0 C0 xs); intro ]
-    end.
-
-  Local Ltac t_reduce_list_evar :=
-    t_prereduce_list_evar;
-    t_postreduce_list.
-
-  Local Ltac t_postreduce_list_with_hyp :=
-    idtac;
-    match goal with
-      | [ |- list_rect ?P ?N ?C (?f ?a) ?a ?b ?c = list_rect ?P ?N' ?C' (?f ?a) ?a ?b ?c ]
-        => let P0 := fresh in
-           let N0 := fresh in
-           let C0 := fresh in
-           let N1 := fresh in
-           let C1 := fresh in
-           set (P0 := P);
-             set (N0 := N);
-             set (C0 := C);
-             set (N1 := N');
-             set (C1 := C');
-             let IH := fresh "IH" in
-             let xs := fresh "xs" in
-             refine (list_rect
-                       (fun ls' => forall a' (pf : ls' = f a') b' c',
-                                     list_rect P0 N0 C0 ls' a' b' c'
-                                     = list_rect P0 N1 C1 ls' a' b' c')
-                       _
-                       _
-                       (f a) a eq_refl b c);
-               simpl @list_rect;
-               [ subst P0 N0 C0 N1 C1; intros; cbv beta
-               | intros ? xs IH; intros; unfold C0 at 1, C1 at 1; cbv beta;
-                 match goal with
-                   | [ |- appcontext[list_rect P0 N1 C1 ?ls'' ?a''] ]
-                     => specialize (IH a'')
-                 end;
-                 let T := match type of IH with ?T -> _ => T end in
-                 let H_helper := fresh in
-                 assert (H_helper : T);
-                   [
-                     | specialize (IH H_helper);
-                       setoid_rewrite <- IH; clear IH N1 C1;
-                       generalize (list_rect P0 N0 C0 xs); intro ] ]
-    end.
-
-  Local Ltac t_postreduce_list_with_hyp_with_assumption :=
-    idtac;
-    lazymatch goal with
-      | [ H : ?HP (?HP' (?f ?a)) = true |- list_rect ?P ?N ?C (?f ?a) ?a ?b ?c = list_rect ?P ?N' ?C' (?f ?a) ?a ?b ?c ]
-        => let P0 := fresh in
-           let N0 := fresh in
-           let C0 := fresh in
-           let N1 := fresh in
-           let C1 := fresh in
-           set (P0 := P);
-             set (N0 := N);
-             set (C0 := C);
-             set (N1 := N');
-             set (C1 := C');
-             let IH := fresh "IH" in
-             let xs := fresh "xs" in
-             let pf := fresh "pf" in
-             refine (list_rect
-                       (fun ls' => forall a' (pf : ls' = f a') (H' : HP (HP' (f a')) = true) b' c',
-                                     list_rect P0 N0 C0 ls' a' b' c'
-                                     = list_rect P0 N1 C1 ls' a' b' c')
-                       _
-                       _
-                       (f a) a eq_refl H b c);
-               simpl @list_rect;
-               [ subst P0 N0 C0 N1 C1; intros; cbv beta
-               | intros ? xs IH pg; intros; unfold C0 at 1, C1 at 1; cbv beta;
-                 match goal with
-                   | [ |- appcontext[list_rect P0 N1 C1 ?ls'' ?a''] ]
-                     => specialize (IH a'')
-                 end;
-                 let T := match type of IH with ?T1 -> ?T2 -> _ => constr:((T1 * T2)%type) end in
-                 let H_helper := fresh in
-                 let H_helper' := fresh in
-                 assert (H_helper : T);
-                   [ split
-                     | specialize (IH (fst H_helper) (snd H_helper));
-                       setoid_rewrite <- IH; clear IH N1 C1;
-                       generalize (list_rect P0 N0 C0 xs); intro ] ]
-    end.
-
-  Local Ltac t_reduce_list_evar_with_hyp :=
-    t_prereduce_list_evar;
-    t_postreduce_list_with_hyp.
-
-  Local Ltac t_refine_item_match_terminal :=
-    idtac;
-    match goal with
-      | [ |- _ = match ?it with Terminal _ => _ | NonTerminal nt => @?NT nt end :> ?T ]
-        => refine (_ : item_rect (fun _ => T) _ NT it = _);
-          revert it;
-          refine (item_rect
-                    _
-                    _
-                    _); simpl @item_rect; intro;
-          [ | reflexivity ]
-    end.
-
-  Local Ltac t_refine_item_match :=
-    idtac;
-    (lazymatch goal with
-      | [ |- _ = match ?it with Terminal _ => _ | _ => _ end :> ?T ]
-        => (refine (_ : item_rect (fun _ => T) _ _ it = _);
-          (lazymatch goal with
-            | [ |- item_rect ?P ?TC ?NC it = match it with Terminal t => @?TC' t | NonTerminal nt => @?NC' nt end ]
-              => refine (item_rect
-                           (fun it' => item_rect (fun _ => T) TC NC it'
-                                       = item_rect (fun _ => T) TC' NC' it')
-                           _
-                           _
-                           it)
-          end;
-          clear it; simpl @item_rect; intro))
-    end).
-
-  Local Arguments Compare_dec.leb !_ !_.
-  Local Arguments to_nonterminal / .
-
-  Local Instance good_nth_proper {A}
-  : Proper (eq ==> _ ==> _ ==> eq) (nth (A:=A))
-    := _.
-  Local Instance good_nth'_proper {A}
-  : Proper (eq ==> _ ==> _ ==> eq) (nth' (A:=A))
-    := _.
-
-  Local Ltac rewrite_map_nth_rhs :=
-    idtac;
-    match goal with
-      | [ |- _ = ?RHS ]
-        => let v := match RHS with
-                      | context[match nth ?n ?ls ?d with _ => _ end]
-                        => constr:(nth n ls d)
-                      | context[nth ?n ?ls ?d]
-                        => constr:(nth n ls d)
-                    end in
-           let P := match (eval pattern v in RHS) with
-                      | ?P _ => P
-                    end in
-           rewrite <- (map_nth P)
-    end.
-
-  Local Ltac rewrite_map_nth_dep_rhs :=
-    idtac;
-    match goal with
-      | [ |- _ = ?RHS ]
-        => let v := match RHS with
-                      | context[match nth ?n ?ls ?d with _ => _ end]
-                        => constr:(nth n ls d)
-                      | context[nth ?n ?ls ?d]
-                        => constr:(nth n ls d)
-                    end in
-           let n := match v with nth ?n ?ls ?d => n end in
-           let ls := match v with nth ?n ?ls ?d => ls end in
-           let d := match v with nth ?n ?ls ?d => d end in
-           let P := match (eval pattern v in RHS) with
-                      | ?P _ => P
-                    end in
-           let P := match (eval pattern n in P) with
-                      | ?P _ => P
-                    end in
-           rewrite <- (map_nth_dep P ls d n)
-    end.
-
-  Local Ltac t_pull_nth :=
-    repeat match goal with
-             | _ => rewrite drop_all by (simpl; omega)
-             | [ |- _ = nth _ _ _ ] => step_opt'
-             | [ |- _ = nth' _ _ _ ] => step_opt'
-             | _ => rewrite !map_map
-             | _ => progress simpl
-             | _ => rewrite <- !surjective_pairing
-             | _ => progress rewrite_map_nth_rhs
-           end;
-    fin_step_opt.
-  Local Ltac t_after_pull_nth_fin :=
-    idtac;
-    match goal with
-      | [ |- appcontext[@nth] ] => fail 1
-      | [ |- appcontext[@nth'] ] => fail 1
-      | _ => repeat step_opt'
-    end.
 
   Let Let_In' {A B} (x : A) (f : forall y : A, B y) : B x
     := let y := x in f y.
@@ -954,14 +204,6 @@ Section recursive_descent_parser.
     exact (proj2_sig (rdp_list_to_production_opt_sig x)).
   Qed.
 
-  Lemma opt_helper_minusr_proof
-  : forall {len0 len}, len <= len0 -> forall n : nat, (len - n)%natr <= len0.
-  Proof.
-    clear.
-    intros.
-    rewrite minusr_minus; omega.
-  Qed.
-
   Definition parse_nonterminal_opt'0
              (str : String)
              (nt : String.string)
@@ -970,108 +212,6 @@ Section recursive_descent_parser.
     exists (parse_nonterminal (data := optdata) str nt).
     reflexivity.
   Defined.
-
-  Local Ltac optsplit_t' :=
-    idtac;
-    match goal with
-      | [ |- _ = ?f match ?v with nil => ?N | x::xs => @?C x xs end ]
-        => let RHS := match goal with |- _ = ?RHS => RHS end in
-           let P := match (eval pattern v in RHS) with ?P _ => P end in
-           transitivity (match v with
-                           | nil => P nil
-                           | x::xs => P (x::xs)
-                         end);
-             [ simpl | destruct v; reflexivity ]
-      | [ |- _ = ?f match ?v with Terminal t => @?T t | NonTerminal nt => @?NT nt end ]
-        => let RHS := match goal with |- _ = ?RHS => RHS end in
-           let P := match (eval pattern v in RHS) with ?P _ => P end in
-           transitivity (match v with
-                           | Terminal t => P (Terminal t)
-                           | NonTerminal nt => P (NonTerminal nt)
-                         end);
-             [ simpl | destruct v; reflexivity ]
-      | [ |- ?e = match ?v with nil => ?N | x::xs => @?C x xs end :> ?T ]
-        => idtac;
-          repeat match goal with
-                 | [ H : context[v] |- _ ]
-                   => hnf in H;
-                     match type of H with
-                     | context[v] => fail 1
-                     | _ => idtac
-                     end
-                 end;
-          let P := match (eval pattern v in T) with ?P _ => P end in
-          change (e = list_caset P N C v);
-            revert dependent v;
-            let NT := type of N in
-            let CT := type of C in
-            let N' := fresh in
-            let C' := fresh in
-            evar (N' : NT);
-              evar (C' : CT);
-              intro v; intros;
-              refine (_ : list_caset P N' C' v = list_caset P N C v);
-              refine (list_caset
-                        (fun v' => list_caset P N' C' v' = list_caset P N C v')
-                        _
-                        _
-                        v);
-              subst N' C'; simpl @list_caset; repeat intro
-      | [ H : is_true (item_rvalid ?G ?v)
-          |- ?e = match ?v with Terminal t => @?T t | NonTerminal nt => @?NT nt end ]
-        => idtac; let TT := type of T in
-                  let NTT := type of NT in
-                  let T' := fresh in
-                  let NT' := fresh in
-                  revert dependent v;
-                    evar (T' : TT);
-                    evar (NT' : NTT);
-                    intro v; intros;
-                    let eqP := match goal with |- _ = _ :> ?P => P end in
-                    let P := match (eval pattern v in eqP) with ?P _ => P end in
-                      change (e = item_rect P T NT v);
-                      refine (_ : item_rect P T' NT' v = item_rect P T NT v);
-                      refine (item_rect
-                                (fun v' => item_rvalid G v' -> item_rect P T' NT' v' = item_rect P T NT v')
-                                _
-                                _
-                                v H);
-                      subst T' NT';
-                      simpl @item_rect; intros ??
-      | [ |- ?e = match ?v with Terminal t => @?T t | NonTerminal nt => @?NT nt end ]
-        => idtac; let TT := type of T in
-                  let NTT := type of NT in
-                  let T' := fresh in
-                  let NT' := fresh in
-                  revert dependent v;
-                    evar (T' : TT);
-                    evar (NT' : NTT);
-                    intro v; intros;
-                    let eqP := match goal with |- _ = _ :> ?P => P end in
-                    let P := match (eval pattern v in eqP) with ?P _ => P end in
-                      change (e = item_rect P T NT v);
-                      refine (_ : item_rect P T' NT' v = item_rect P T NT v);
-                      refine (item_rect
-                                (fun v' => item_rect P T' NT' v' = item_rect P T NT v')
-                                _
-                                _
-                                v);
-                      subst T' NT';
-                      simpl @item_rect; intro
-      | [ |- _ = _::_ ] => etransitivity_rev (_::_);
-                          [ apply f_equal2
-                          | reflexivity ]
-      | _ => progress fin_step_opt
-    end.
-
-  Local Ltac change_char_at_matches :=
-    idtac;
-    lazymatch goal with
-    | [ |- appcontext G[@char_at_matches ?Char ?HSLM ?n ?str (@interp_RCharExpr _ ?data ?P)] ]
-      => idtac;
-         let G' := context G[@char_at_matches_interp Char HSLM data n str P] in
-         change G'
-    end.
 
   Definition parse_nonterminal_opt'1
              (str : String)
@@ -1230,7 +370,7 @@ Section recursive_descent_parser.
                    | _ => progress simpl
                    end. } }
         simpl.
-        step_opt'; [ reflexivity | | reflexivity ].
+        step_opt'; [ | reflexivity ].
         etransitivity_rev _.
         { move Hvalid''' at bottom.
           simpl @to_production in Hvalid'''.
@@ -1412,7 +552,7 @@ Section recursive_descent_parser.
         etransitivity_rev _.
         { step_opt'.
           etransitivity_rev _.
-          { repeat step_opt'; [ reflexivity | | reflexivity ].
+          { repeat step_opt'; [ | reflexivity ].
             rewrite nth'_nth.
             rewrite_map_nth_rhs; rewrite !map_map; simpl.
             rewrite <- nth'_nth.
@@ -1447,19 +587,13 @@ Section recursive_descent_parser.
             lazymatch goal with
             | [ |- _ = bool_rect ?P (if ?b then ?t else ?f) ?t ?b' ]
               => transitivity (if (orb (negb b') b) then t else f); [ | destruct b, b'; reflexivity ]
-            end.
-            apply (f_equal3 (fun (b : bool) x y => if b then x else y)); [ | reflexivity | reflexivity ]. (*
+            end; fin_step_opt.
             match goal with
             | [ |- context[negb (EqNat.beq_nat ?x 0)] ]
-              => replace (negb (EqNat.beq_nat x 0)) with (Compare_dec.leb
-let z := fresh in
-                 let y' := fresh in
-                 set (z := x);
-                   set (y' := y);
-                   refine (_ : orb (Compare_dec.leb 1 x) y = _);
-                   change (orb (Compare_dec.leb 1 z) y' = orb (negb (EqNat.beq_nat z 0)) (andb (EqNat.beq_nat z 0) y'));
-                   destruct z, y'; reflexivity
-            end. }
+              => replace (negb (EqNat.beq_nat x 0)) with (Compare_dec.leb 1 x)
+                by (destruct x as [|[]]; reflexivity)
+            end.
+            reflexivity. }
           etransitivity_rev _.
           { apply (f_equal2 (inner_nth' _)); [ | reflexivity ].
             step_opt'; [ ].
@@ -1469,20 +603,21 @@ let z := fresh in
             rewrite <- nth'_nth.
             change @nth' with @inner_nth' at 1.
             reflexivity. }
-          reflexivity. }
-        (*etransitivity_rev _.
-        { change @inner_nth' with @nth' at 1.
           etransitivity_rev _.
-          { step_opt'.
-            etransitivity_rev _.
-            { step_opt'.
-              rewrite nth'_nth; reflexivity. }
+          { apply (f_equal2 (inner_nth' _)); [ | reflexivity ].
+            step_opt'.
+            apply (f_equal2 (inner_nth' _)); [ reflexivity | ].
+            lazymatch goal with
+            | [ |- _ = bool_rect ?P (if ?b then ?t else ?f) ?t ?b' ]
+              => transitivity (if (orb (negb b') b) then t else f); [ | destruct b, b'; reflexivity ]
+            end; fin_step_opt.
             match goal with
-              | [ |- _ = map (fun x => nth ?n (@?ls x) ?d) ?ls' ]
-                => etransitivity_rev (map (fun ls'' => nth n ls'' d) (map ls ls'));
-                  [ rewrite !map_map; reflexivity | ]
+            | [ |- context[negb (EqNat.beq_nat ?x 0)] ]
+              => replace (negb (EqNat.beq_nat x 0)) with (Compare_dec.leb 1 x)
+                by (destruct x as [|[]]; reflexivity)
             end.
-            reflexivity. }*)
+            reflexivity. }
+          reflexivity. }
         reflexivity. }
       reflexivity. }
     etransitivity_rev _.
@@ -1526,29 +661,36 @@ let z := fresh in
 
         step_opt'; [].
         step_opt'.
-        { set_evars.
-          setoid_rewrite combine_map_r.
-          do 2 setoid_rewrite map_map; simpl.
-          setoid_rewrite map_length.
-          progress change (fun x : ?A * ?B => fst x) with (@fst A B).
-          subst_evars.
+        { etransitivity_rev _.
+          { set_evars.
+            do 2 setoid_rewrite combine_map_r.
+            do 3 setoid_rewrite map_map; simpl.
+            setoid_rewrite map_length.
+            progress change (fun x : ?A * ?B => fst x) with (@fst A B).
+            subst_evars.
 
+            reflexivity. }
+
+          refine (f_equal2 ret_production_cons _ _); [ | reflexivity ].
+          apply (_ : Proper (pointwise_relation _ _ ==> _ ==> _ ==> _) (ritem_rect (fun _ => parse_item_T))); repeat intro;
+            [ | reflexivity | reflexivity ].
+          change_char_at_matches.
           reflexivity. }
         { set_evars.
-          setoid_rewrite combine_map_r.
+          do 2 setoid_rewrite combine_map_r.
           subst_evars.
 
           step_opt'.
           { set_evars.
-            do 2 setoid_rewrite map_map; simpl.
+            change_char_at_matches.
+            do 3 setoid_rewrite map_map; simpl.
             setoid_rewrite map_length.
-            rewrite !Nat.add_1_r.
             subst_evars.
 
             reflexivity. }
           { step_opt'; [ | reflexivity ].
             set_evars.
-            do 2 setoid_rewrite map_map; simpl.
+            do 3 setoid_rewrite map_map; simpl.
             setoid_rewrite map_length.
             progress change (fun x : ?A * ?B => fst x) with (@fst A B).
             subst_evars.
@@ -1557,560 +699,42 @@ let z := fresh in
       { reflexivity. } }
 
     simpl.
-    reflexivity.
-  Defined.
+    progress change (fun x : list ?T => @List.length ?T x) with (@List.length T).
+    progress change @inner_nth' with @nth'.
 
-  Definition parse_nonterminal_opt'2
-             (str : String)
-             (nt : String.string)
-  : { b : bool | b = parse_nonterminal (data := optdata) str nt }.
-  Proof.
-    let c := constr:(parse_nonterminal_opt'1 str nt) in
-    let h := head c in
-    let p := (eval cbv beta iota zeta delta [proj1_sig h] in (proj1_sig c)) in
-    sigL_transitivity p; [ | abstract exact (proj2_sig c) ].
-    refine_Fix2_5_Proper_eq.
-    etransitivity_rev _.
-    { fix2_trans;
-      [
-      | solve [ change @opt3.nth' with @nth';
-                change @opt2.map with @List.map;
-                change @inner_nth' with @nth';
-                t_reduce_fix;
-                t_postreduce_list;
-                unfold ritem_rect;
-                t_reduce_fix ] ].
-      reflexivity. }
-
-    (** [nth'] is useful when the index is unknown at top-level, but performs poorly in [simpl] when the index is eventually known at compile-time.  So we need to remove the [nth'] *)
-    etransitivity_rev _.
-    { change @inner_nth' with @nth'.
-      step_opt'; [ | reflexivity ].
-      step_opt'; [].
-      apply (f_equal2 (nth' _)); [ | reflexivity ].
-      step_opt'; [ | reflexivity ].
-      step_opt'; [].
-      rewrite !nth'_nth; apply (f_equal2 (nth _)); [ | ].
-      { step_opt'; [ ].
-        rewrite !nth'_nth; apply (f_equal2 (nth _)); [ | ].
-        { step_opt'; [].
-          match goal with
-          | [ |- _ = @bool_rect (fun _ => ?P) _ _ _ ]
-            => apply (f_equal3 (bool_rect (fun _ => P)))
-          end; [ reflexivity | | ];
-          fin_step_opt.
-          { t_reduce_list_evar; [ reflexivity | ].
-            step_opt'; [].
-            step_opt'; [ | ].
-            { rewrite nth'_nth.
-              rewrite <- andbr_andb at 1.
-              apply (f_equal2 andbr).
-              { match goal with
-                | [ |- _ = ?f ?x ?a ?b ]
-                  => refine (f_equal (fun x' => f x' a b) _)
-                end.
-                fin_step_opt; [ reflexivity | ].
-                apply (f_equal2 (nth _)); [ | reflexivity ].
-                step_opt'; [ | reflexivity ].
-                rewrite nth'_nth; reflexivity. }
-              { step_opt'; [ | reflexivity ].
-                change_char_at_matches.
-                reflexivity. } }
-            { step_opt'.
-              { rewrite <- andbr_andb at 1.
-                apply (f_equal2 andbr); [ | ].
-                { change_char_at_matches.
-                  reflexivity. }
-                { rewrite nth'_nth.
-                  match goal with
-                  | [ |- _ = ?f ?x ?a ?b ]
-                    => refine (f_equal (fun x' => f x' a b) _)
-                  end.
-                  fin_step_opt; [ reflexivity | ].
-                  apply (f_equal2 (nth _)); [ | reflexivity ].
-                  step_opt'; [ | reflexivity ].
-                  rewrite nth'_nth; reflexivity. } }
-              { step_opt'; [ | reflexivity ].
-                apply (f_equal2 andb); [ reflexivity | ].
-                rewrite nth'_nth.
-                match goal with
-                | [ |- _ = ?f ?x ?a ?b ]
-                  => refine (f_equal (fun x' => f x' a b) _)
-                end.
-                fin_step_opt; [ reflexivity | ].
-                apply (f_equal2 (nth _)); [ | reflexivity ].
-                step_opt'; [ | reflexivity ].
-                rewrite nth'_nth; reflexivity. } } }
-          { apply (f_equal2 (nth _)); [ | reflexivity ].
-            step_opt'; [ ].
-            step_opt'; [ progress simpl ].
-            rewrite nth'_nth.
-            apply (f_equal2 (nth _)); [ | reflexivity ].
-            reflexivity. } }
-        { etransitivity_rev _.
-          { rewrite bool_rect_andb.
-            rewrite Bool.andb_true_r.
-            match goal with
-            | [ |- _ = (orb (negb (EqNat.beq_nat ?x 0)) (andb (EqNat.beq_nat ?x 0) ?y)) ]
-              => let z := fresh in
-                 let y' := fresh in
-                 set (z := x);
-                   set (y' := y);
-                   refine (_ : orb (Compare_dec.leb 1 x) y = _);
-                   change (orb (Compare_dec.leb 1 z) y' = orb (negb (EqNat.beq_nat z 0)) (andb (EqNat.beq_nat z 0) y'));
-                   destruct z, y'; reflexivity
-            end. }
-          apply (f_equal2 orb); fin_step_opt; [].
-          apply (f_equal2 (nth _)); [ | reflexivity ].
-          step_opt'; [ ].
-          step_opt'; [ progress simpl ].
-          rewrite nth'_nth.
-          apply (f_equal2 (nth _)); [ | reflexivity ].
-          reflexivity. } }
-      { apply (f_equal2 orb); fin_step_opt; [].
-        apply (f_equal2 (nth _)); [ | reflexivity ].
-        step_opt'; [ ].
-        step_opt'; [ progress simpl ].
-        rewrite nth'_nth.
-        apply (f_equal2 (nth _)); [ | reflexivity ].
-        reflexivity. } }
-    change @nth' with @inner_nth' at 1.
-    match goal with
-      | [ |- appcontext[@nth'] ] => fail 1
-      | _ => change @inner_nth' with @nth'
-    end.
+    (** change [nth'] back to [nth] *)
     etransitivity_rev _.
     { step_opt'; [ | reflexivity ].
-      rewrite nth'_nth at 1.
-      rewrite_map_nth_rhs; rewrite !map_map; simpl.
-      rewrite <- nth'_nth at 1.
-      reflexivity. }
+      step_opt'.
+      step_opt'.
+      apply (f_equal2 (nth' _)); fin_step_opt; [].
+      repeat lazymatch goal with
+             | [ |- _ = nth' _ _ _ ]
+               => rewrite nth'_nth; apply (f_equal2 (nth _))
+             | [ |- _ = orb _ _ ] => apply f_equal2
+             | [ |- _ = ret_production_cons _ _ ] => apply f_equal2
+             | [ |- _ = list_rect _ _ _ ?x _ _ _ ]
+               => is_var x; t_reduce_list_evar
+             | [ |- _ = ?f (_, (_, _)) _ _ ]
+               => is_var f; apply f_equal3
+             | [ |- appcontext[@nth'] ]
+               => step_opt' || fin_step_opt
+             | _ => reflexivity
+             end. }
 
+    simpl.
     reflexivity.
   Defined.
 
-  Local Ltac safe_change_opt' :=
-    idtac;
-    match goal with
-    | [ |- context G[minusr (opt.id ?x) (opt.id ?y)] ]
-      => let G' := context G[opt.id (opt.minusr x y)] in
-         change G'
-    | [ |- context G[minusr (opt.id ?x) (opt2.id ?y)] ]
-      => let G' := context G[opt2.id (opt2.minusr x y)] in
-         change G'
-    | [ |- context G[fst (opt.id ?x)] ]
-      => let G' := context G[opt.id (opt.fst x)] in
-         change G'
-    | [ |- context G[snd (opt.id ?x)] ]
-      => let G' := context G[opt.id (opt.snd x)] in
-         change G'
-    | [ |- context G[fst (opt2.id ?x)] ]
-      => let G' := context G[opt2.id (opt2.fst x)] in
-         change G'
-    | [ |- context G[snd (opt2.id ?x)] ]
-      => let G' := context G[opt2.id (opt2.snd x)] in
-         change G'
-    | [ |- appcontext G[nth (opt2.id ?x) ?ls ?d] ]
-      => let G' := context G[opt2.id (opt2.nth x ls d)] in
-         change G'
-    | [ |- context G[StringLike.length (opt.id ?str)] ]
-      => let G' := context G[StringLike.length str] in
-         change G'
-    | [ |- context G[map (opt.id ?f) (opt.id ?x)] ]
-      => let G' := context G[opt.id (opt.map f x)] in
-         change G'
-    | [ |- context G[map fst (opt.id ?x)] ]
-      => let G' := context G[opt.id (opt.map opt.fst x)] in
-         change G'
-    | [ |- context G[map snd (opt.id ?x)] ]
-      => let G' := context G[opt.id (opt.map opt.snd x)] in
-         change G'
-    (*| [ |- appcontext G[snd (of_string (opt.id ?x))] ]
-               => let G' := context G[opt.snd (of_string x)] in
-                  change G'*)
-    | [ |- context G[string_beq (opt.id ?x)] ]
-      => let G' := context G[opt.id (opt.string_beq x)] in
-         change G'
-    | [ |- context G[fun x0 y0 : ?T => string_beq (fst x0) (fst y0)] ]
-      => let G' := context G[opt.id (fun x0 y0 : T => opt.string_beq (opt.fst x0) (opt.fst y0))] in
-         change G'
-    | [ |- context G[uniquize (opt.id ?beq) (opt.id ?ls)] ]
-      => let G' := context G[opt.id (opt.uniquize beq ls)] in
-         change G'
-    | [ |- context G[uniquize string_beq (opt.id ?ls)] ]
-      => let G' := context G[opt.id (opt.uniquize opt.string_beq ls)] in
-         change G'
-    | [ |- context G[List.length (opt.id ?ls)] ]
-      => let G' := context G[opt.id (opt.length ls)] in
-         change G'
-    | [ |- context G[List.length (opt2.id ?ls)] ]
-      => let G' := context G[opt2.id (opt2.length ls)] in
-         change G'
-    | [ |- context G[first_index_default (opt.id ?x) (opt.id ?y) (opt.id ?z)] ]
-      => let G' := context G[opt.id (opt.first_index_default x y z)] in
-         change G'
-    | [ |- context G[up_to (opt.id ?n)] ]
-      => let G' := context G[opt.id (opt.up_to n)] in
-         change G'
-    | [ |- context G[pred (opt.id ?n)] ]
-      => let G' := context G[opt.id (opt.pred n)] in
-         change G'
-    | [ |- context G[rev (opt.id ?ls)] ]
-      => let G' := context G[opt.id (opt.rev ls)] in
-         change G'
-    | [ |- context G[fun x0 : ?T => up_to (Datatypes.length (snd x0))] ]
-      => let G' := context G[opt.id (fun x0 : T => opt.up_to (opt.length (opt.snd x0)))] in
-         change G'
-    | [ |- context G[combine (opt.id ?ls) (opt.id ?ls')] ]
-      => let G' := context G[opt.id (opt.combine ls ls')] in
-         change G'
-    | [ |- context G[List.hd ?d (opt.id ?ls)] ]
-      => let G' := context G[opt.id (opt.hd d ls)] in
-         change G'
-    | [ |- context G[fst (of_string ?str')] ]
-      => let G' := context G[opt.id (opt.fst (of_string str'))] in
-         change G'
-    | [ |- context G[snd (of_string ?str')] ]
-      => let G' := context G[opt.id (opt.snd (of_string str'))] in
-         change G'
-    | [ |- context G[EqNat.beq_nat (opt2.id ?x) 0] ]
-      => let G' := context G[opt2.id (opt2.beq_nat x 0)] in
-         change G'
-    | [ |- context G[(opt2.id ?x, 0)] ]
-      => let G' := context G[opt2.id (x, 0)] in
-         change G'
-    | [ |- context G[(opt2.id ?x, opt2.id ?y)] ]
-      => let G' := context G[opt2.id (x, y)] in
-         change G'
-    | [ |- context G[EqNat.beq_nat (opt.id ?x) 0] ]
-      => let G' := context G[opt.id (opt.beq_nat x 0)] in
-         change G'
-    | [ |- context G[S (opt2.id ?x)] ]
-      => let G' := context G[opt2.id (S x)] in
-         change G'
-    | [ |- context G[S (opt.id ?x)] ]
-      => let G' := context G[opt.id (S x)] in
-         change G'
-    | [ |- context G[Compare_dec.leb (opt2.id ?x) (opt.id ?y)] ]
-      => let G' := context G[opt2.id (opt2.leb x y)] in
-         change G'
-    | [ |- context G[Compare_dec.leb 1 (opt2.id ?x)] ]
-      => let G' := context G[opt2.id (opt2.leb 1 x)] in
-         change G'
-    | [ |- context G[Compare_dec.leb 1 (opt2.length ?x)] ]
-      => let G' := context G[opt2.id (opt2.leb 1 (opt2.length x))] in
-         change G'
-    | [ |- context G[@interp_RCharExpr ?Char ?idata (opt.id ?expr)] ]
-      => let G' := context G[opt.id (@opt.interp_RCharExpr Char idata expr)] in
-         change G'
-    end.
-
-  Local Ltac change_opt_reduce' :=
-    idtac;
-    match goal with
-    | _ => progress safe_change_opt'
-    | [ |- ?LHS = _ ]
-      => match LHS with
-         | appcontext[opt.id] => unfold opt.id at 1
-         | appcontext[opt2.id] => unfold opt2.id at 1
-         | appcontext[opt3.id] => unfold opt3.id at 1
-         end
-    | [ |- ?e = opt.id ?x ]
-      => progress change (e = x)
-    | [ |- ?e = opt2.id ?x ]
-      => progress change (e = x)
-    | [ |- _ = opt2.map _ _ ]
-      => apply ((_ : Proper (pointwise_relation _ _ ==> eq ==> eq) (@List.map _ _))
-                : Proper (pointwise_relation _ _ ==> eq ==> eq) (@opt2.map _ _));
-        [ let x := fresh in intro x; change x with (opt2.id x)
-        | ]
-    | [ |- _ = opt.map _ _ ]
-      => apply ((_ : Proper (pointwise_relation _ _ ==> eq ==> eq) (@List.map _ _))
-                : Proper (pointwise_relation _ _ ==> eq ==> eq) (@opt.map _ _));
-        [ let x := fresh in intro x; change x with (opt.id x)
-        | ]
-    | [ |- _ = @opt.fold_left ?A ?B orb _ false ]
-      => refine (_ : opt.fold_left orb _ false = _);
-        apply ((_ : Proper (_ ==> _ ==> _ ==> _) (@fold_left A B))
-               : Proper _ (@opt.fold_left A B));
-        repeat (let x := fresh in intro x; change x with (opt.id x))
-    | [ |- _ = @opt.fold_left ?A ?B orbr _ false ]
-      => refine (_ : opt.fold_left orbr _ false = _);
-        apply ((_ : Proper (_ ==> _ ==> _ ==> _) (@fold_left A B))
-               : Proper _ (@opt.fold_left A B));
-        repeat (let x := fresh in intro x; change x with (opt.id x))
-    | [ |- _ = @opt.list_caset ?A (fun _ => ?P) _ _ _ ]
-      => refine (_ : @opt.list_caset A (fun _ => P) _ _ _ = _);
-        apply ((_ : Proper (_ ==> pointwise_relation _ (pointwise_relation _ _) ==> _ ==> _) (@list_caset A (fun _ => P)))
-               : Proper _ (@opt.list_caset A (fun _ => P)));
-        repeat (let x := fresh in intro x; change x with (opt.id x))
-    | _ => progress cbv beta
-    | [ |- _ = opt2.nth _ _ _ ]
-      => apply (f_equal2 (opt2.nth _))
-    | [ |- _ = opt2.bool_rect ?P _ _ _ ]
-      => apply (f_equal3 (opt2.bool_rect P))
-    | _ => progress fin_step_opt
-    | [ |- _ = orb _ _ ] => apply (f_equal2 orb)
-    | [ |- _ = orbr _ _ ] => apply (f_equal2 orbr)
-    | [ |- _ = andb _ _ ] => apply (f_equal2 andb)
-    | [ |- _ = andbr _ _ ] => apply (f_equal2 andbr)
-    | [ |- _ = minusr _ _ ] => apply (f_equal2 minusr)
-    | [ |- ?e = List.map ?f (opt2.id ?x) ]
-      => progress change (e = opt2.map f x)
-    | [ |- context G[List.map ?f (opt.id ?ls)] ]
-      => let G' := context G[opt.id (opt.map f ls)] in
-         change G'
-    | [ |- context G[bool_rect ?x ?y ?z (opt.id ?w)] ]
-      => let G' := context G[opt.id (opt.bool_rect x y z w)] in
-         change G'
-    | [ |- context G[bool_rect ?x ?y ?z (opt2.id ?w)] ]
-      => let G' := context G[opt2.id (opt2.bool_rect x y z w)] in
-         change G'
-    | [ |- context G[list_caset ?x ?y ?z (opt.id ?w)] ]
-      => let G' := context G[opt.id (opt.list_caset x y z w)] in
-         change G'
-    | [ |- context G[item_rect ?x ?y ?z (opt.id ?w)] ]
-      => let G' := context G[opt.id (opt.item_rect x y z w)] in
-         change G'
-    | [ |- context G[ritem_rect ?x ?y ?z (opt.id ?w)] ]
-      => let G' := context G[opt.id (opt.ritem_rect x y z w)] in
-         change G'
-    | [ |- context G[List.fold_left orb (opt.id ?ls) false] ]
-      => let G' := context G[opt.id (opt.fold_left orb ls false)] in
-         change G'
-    | [ |- context G[List.fold_left orbr (opt.id ?ls) false] ]
-      => let G' := context G[opt.id (opt.fold_left orbr ls false)] in
-         change G'
-    | [ |- _ = list_rect ?P ?N ?C (opt.id ?ls) (opt2.id ?idx) ?offset ?len ]
-      => t_reduce_list_evar;
-        [
-               | match goal with
-                 | [ |- ?e ?x ?xs ?H ?a ?b ?c = _ ]
-                   => is_evar e;
-                     change x with (opt.id x);
-                     change xs with (opt.id xs);
-                     change a with (opt2.id a)
-                 end ]
-    | [ |- _ = opt.item_rect ?T ?A ?B ?c ] (* evar kludge following *)
-      => revert c;
-        let RHS := match goal with |- forall c', _ = ?RHS c' => RHS end in
-        let f := constr:(fun TC NC =>
-                           forall c, opt.item_rect T TC NC c = RHS c) in
-        let f := (eval cbv beta in f) in
-        let e1 := fresh in
-        let e2 := fresh in
-        match type of f with
-        | ?X -> ?Y -> _
-          => evar (e1 : X); evar (e2 : Y)
-        end;
-          intro c;
-          let ty := constr:(opt.item_rect T e1 e2 c = RHS c) in
-          etransitivity_rev _; [ refine (_ : ty) | reflexivity ];
-          revert c;
-          refine (item_rect
-                    (fun c => opt.item_rect T e1 e2 c = RHS c)
-                    _ _);
-          intro c; simpl @opt.item_rect; subst e1 e2;
-          change c with (opt.id c)
-    | [ |- _ = opt.ritem_rect ?T ?A ?B ?c ] (* evar kludge following *)
-      => revert c;
-        let RHS := match goal with |- forall c', _ = ?RHS c' => RHS end in
-        let f := constr:(fun TC NC =>
-                           forall c, opt.ritem_rect T TC NC c = RHS c) in
-        let f := (eval cbv beta in f) in
-        let e1 := fresh in
-        let e2 := fresh in
-        match type of f with
-        | ?X -> ?Y -> _
-          => evar (e1 : X); evar (e2 : Y)
-        end;
-          intro c;
-          let ty := constr:(opt.ritem_rect T e1 e2 c = RHS c) in
-          etransitivity_rev _; [ refine (_ : ty) | reflexivity ];
-          revert c;
-          refine (ritem_rect
-                    (fun c => opt.ritem_rect T e1 e2 c = RHS c)
-                    _ _);
-          intro c; simpl @opt.ritem_rect; subst e1 e2;
-          change c with (opt.id c)
-    | [ |- _ = opt2.beq_nat _ _ ] => apply (f_equal2 opt2.beq_nat)
-    | [ |- _ = opt2.leb _ _ ] => apply (f_equal2 opt2.leb)
-    | [ |- _ = opt2.length _ ] => apply f_equal
-    | [ |- _ = opt.snd _ ] => apply f_equal
-    | [ |- _ = opt2.snd _ ] => apply f_equal
-    | [ |- _ = opt.fst _ ] => apply f_equal
-    | [ |- _ = opt2.fst _ ] => apply f_equal
-    | [ |- _ = opt.interp_RCharExpr _ ] => apply f_equal
-    | [ |- _ = opt.uniquize _ _ ] => reflexivity
-    | [ |- _ = opt.combine _ _ ] => reflexivity
-    | [ |- _ = opt.length ?x ] => is_var x; reflexivity
-    | [ |- _ = char_at_matches _ _ _ ] => apply f_equal3
-    | [ |- _ = char_at_matches_interp _ _ _ ] => apply f_equal3
-    end.
-
-  Local Ltac safe_change_opt := repeat safe_change_opt'.
-  Local Ltac change_opt_reduce := repeat change_opt_reduce'.
-
-  Local Ltac do_flip_map ls :=
-    idtac;
-    progress
-      (repeat let A := match goal with |- appcontext[@List.map ?A ?B] => A end in
-              let B := match goal with |- appcontext[@List.map A ?B] => B end in
-              let flip_map := fresh "flip_map" in
-              pose (flip_map ls' f := @List.map A B f ls');
-                progress change (@List.map A B) with (fun f ls' => @flip_map ls' f);
-                cbv beta;
-                try change (@flip_map ls) with (@flip_map (opt.id ls)));
-    repeat match goal with
-           | [ flip_map := fun ls' f => @List.map _ _ f ls' |- _ ]
-             => subst flip_map
-           end;
-    cbv beta.
-
-  Local Ltac do_flip_combine ls :=
-    idtac;
-    progress
-      (repeat let A := match goal with |- appcontext[@List.combine ?A ?B] => A end in
-              let B := match goal with |- appcontext[@List.combine A ?B] => B end in
-              let flip_combine := fresh "flip_combine" in
-              pose (flip_combine ls' f := @List.combine A B f ls');
-                progress change (@List.combine A B) with (fun f ls' => @flip_combine ls' f);
-                cbv beta;
-                try change (@flip_combine ls) with (@flip_combine (opt.id ls)));
-    repeat match goal with
-           | [ flip_combine := fun ls' f => @List.combine _ _ f ls' |- _ ]
-             => subst flip_combine
-           end;
-    cbv beta.
-
-  Definition parse_nonterminal_opt'3
-             (str : String)
-             (nt : String.string)
-  : { b : bool | b = parse_nonterminal (data := optdata) str nt }.
-  Proof.
-    let c := constr:(parse_nonterminal_opt'2 str nt) in
-    let h := head c in
-    let p := (eval cbv beta iota zeta delta [proj1_sig h] in (proj1_sig c)) in
-    sigL_transitivity p; [ | abstract exact (proj2_sig c) ].
-    evar (b' : bool).
-    sigL_transitivity b'; subst b'.
-    Focus 2.
-    { progress unfold rdp_list_of_nonterminal; simpl.
-      unfold pregrammar_nonterminals; simpl.
-      match goal with
-        | [ |- _ = ?f ?x ]
-          => set (F := f)
-      end.
-      rewrite map_length.
-      subst F.
-      (** TODO: Come up with a robust (possibly reflective) version of
-      this, based or wheich things are recursively accessible *)
-      change @nth' with @opt3.nth' at 1.
-      change @List.map with @opt2.map at 1.
-      change (pregrammar_productions G) with (opt.id (pregrammar_productions G)).
-      change nt with (opt.id nt).
-      change str with (opt.id str).
-      safe_change_opt.
-      change (opt.id (pregrammar_productions G)) with (pregrammar_productions G).
-      change (opt.id nt) with nt.
-      change (opt.id str) with str.
-      reflexivity. }
-    Unfocus.
-    refine_Fix2_5_Proper_eq.
-    etransitivity_rev _.
-    { fix2_trans;
-      [
-      | solve [ change @opt3.nth' with @nth';
-                change @opt2.map with @List.map;
-                t_reduce_fix;
-                t_postreduce_list;
-                unfold ritem_rect;
-                t_reduce_fix ] ].
-
-      do_flip_map (pregrammar_rproductions G).
-      do_flip_combine (pregrammar_rproductions G).
-      change (List.length (pregrammar_rproductions G)) with (opt.id (opt.length (pregrammar_rproductions G))).
-
-      step_opt'; [ | reflexivity ].
-      apply (f_equal2 (opt3.nth' _)); [ | reflexivity ].
-      change_opt_reduce.
-      step_opt';
-        change_opt_reduce; [ | | | ].
-      { match goal with
-        | [ |- _ = ?f (opt2.id ?x) ?y ?z ]
-          => refine (f_equal (fun x' => f x' y z) _)
-        end.
-        change_opt_reduce; [].
-        match goal with
-        | [ |- _ = if opt2.id _ then opt2.id _ else opt2.id _ ]
-          => unfold opt2.id; reflexivity
-        end. }
-      { match goal with
-        | [ |- _ = ?f _ _ (opt.id (opt.first_index_default _ _ _)) ]
-          => unfold opt.id
-        end.
-        reflexivity. }
-      { match goal with
-        | [ |- _ = ?f (opt2.id ?x) ?y ?z ]
-          => refine (f_equal (fun x' => f x' y z) _)
-        end.
-        change_opt_reduce; [].
-        match goal with
-        | [ |- _ = if opt2.id _ then opt2.id _ else opt2.id _ ]
-          => unfold opt2.id; reflexivity
-        end. }
-      { change @List.map with @opt2.map at 1. (** FIXME: is this right? *)
-        change_opt_reduce; [ | | progress unfold opt2.id; reflexivity ].
-        { match goal with
-          | [ |- _ = ?f _ _ (opt.id (opt.first_index_default _ _ _)) ]
-            => unfold opt.id
-          end.
-          reflexivity. }
-        { match goal with
-          | [ |- _ = ?f (opt2.id ?x) ?y ?z ]
-            => refine (f_equal (fun x' => f x' y z) _)
-          end.
-          change_opt_reduce; [].
-          match goal with
-          | [ |- _ = if opt2.id _ then opt2.id _ else opt2.id _ ]
-            => unfold opt2.id; reflexivity
-          end. } } }
-    change @fold_left with @opt3.fold_left at 1.
-    change @list_rect with @opt.list_rect at 1.
-    reflexivity.
-  Defined.
-
-  Definition parse_nonterminal_preopt
-             (str : String)
-             (nt : String.string)
-  : { b : bool | b = parse_nonterminal (data := optdata) str nt }.
-  Proof.
-    let c := constr:(parse_nonterminal_opt'2 str nt) in
-    let h := head c in
-    let impl := (eval cbv beta iota zeta delta [h proj1_sig] in (proj1_sig c)) in
-    (exists impl);
-      abstract (exact (proj2_sig c)).
-  Defined.
-
-  Lemma parse_nonterminal_preopt_eq
-        {HSLP : StringLikeProperties Char}
-        {splitdata_correct : @boolean_parser_completeness_dataT' _ _ _ G data}
-        (str : String)
-        (nt : String.string)
-    : proj1_sig (parse_nonterminal_preopt str nt) = parse_nonterminal (data := data) str nt.
-  Proof.
-    rewrite <- parse_nonterminal_optdata_eq.
-    apply proj2_sig.
-  Qed.
 
   Definition parse_nonterminal_opt
              (str : String)
              (nt : String.string)
-  : { b : bool | b = parse_nonterminal (data := optdata) str nt }.
+  : { b : _ | b = parse_nonterminal (data := optdata) str nt }.
   Proof.
-    let c := constr:(parse_nonterminal_opt'3 str nt) in
+    let c := constr:(parse_nonterminal_opt'1 str nt) in
     let h := head c in
-    let impl := (eval cbv beta iota zeta delta [h proj1_sig item_rect ritem_rect list_caset] in (proj1_sig c)) in
+    let impl := (eval cbv beta iota zeta delta [h proj1_sig] in (proj1_sig c)) in
     (exists impl);
       abstract (exact (proj2_sig c)).
   Defined.
@@ -2120,10 +744,10 @@ let z := fresh in
         {splitdata_correct : @boolean_parser_completeness_dataT' _ _ _ G data}
         (str : String)
         (nt : String.string)
-    : proj1_sig (parse_nonterminal_opt str nt) = parse_nonterminal (data := data) str nt.
+    : is_correct (proj1_sig (parse_nonterminal_opt str nt)) str nt.
   Proof.
-    rewrite <- parse_nonterminal_optdata_eq.
-    apply proj2_sig.
+    let p := match goal with |- context[proj1_sig ?p] => p end in
+    rewrite (proj2_sig p).
+    apply parse_nonterminal_optdata_eq.
   Qed.
 End recursive_descent_parser.
-*)
